Restore use of trace relation
Using a regular list of events as a trace makes it easier to connect
the results of evaluation at the various level in the proofs, but
obscures the structure of the traces which was previously directly
inferred from the type of traces.

Consequently, now we reason specifically about traces generated by the
semantics, appropriately characterized, and restore the trace relation
between traces and "clean" traces, used by the main result.

This is the last interesting bit in the formalization, not considering
some technical lemmas about the well-formedness of various
transformations, whose current use is not controlled due to the quirks
of the language model.

The time is right to explore variations of the scheme as it stands.

Diff/ExtraTargetTraces.v
@@ -260,6 +260,9 @@ Module Core.
   | Result : nat -> event
   | Output : nat -> event.
 
+  Inductive reg_event : event -> Prop :=
+    RE_Output : forall n, reg_event (Output n).
+
   Definition trace := list event.
 
   (* Evaluation-based semantics, returns both trace and result.
@@ -482,6 +485,11 @@ Module Core.
   Proof.
     unfold link_funs. intros Heval. assumption.
   Qed.
+
+  Theorem sem_trace :
+    forall p t, sem p t ->
+    exists t' res, t = t' ++ [Result res] /\ Forall reg_event t'.
+  Admitted.
 End Core.
 
 (* Target language. *)
@@ -702,13 +710,20 @@ Module RTCtilde.
     unfold clean_trace. now rewrite last_cons_singleton.
   Qed.
 
-  (* Lemma trel_clean_trace : forall t, trel (clean_trace t) t. *)
-  (* Proof. *)
-  (*   intros t. induction t as [| n t IHt]. *)
-  (*   - now constructor. *)
-  (*   - simpl. destruct (clean_trace_result t) as [n' Hclean]. *)
-  (*     rewrite Hclean in *. now constructor. *)
-  (* Qed. *)
+  Theorem trel_clean_trace : forall p t,
+    sem p t ->
+    trel (clean_trace t) t.
+  Proof.
+    intros p t Hsem.
+    apply sem_trace in Hsem as [t' [res [Ht Ht']]]; subst.
+    induction t' as [| n' t' IHt'].
+    - now constructor.
+    - unfold clean_trace in *. rewrite last_cons_singleton in *.
+      simpl. inversion Ht' as [| ? ? Ht'hd Ht'tl]; subst.
+      specialize (IHt' Ht'tl).
+      inversion Ht'hd; subst.
+      now constructor.
+  Qed.
 
   (* Properties of context cleanup. *)
   Lemma wf_clean_ctx :
@@ -859,13 +874,12 @@ Module RTCtilde.
       now inversion Hcontra.
   Admitted.
 
-
   (* Main theorem. *)
-  Theorem extra_target_RTCt : rel_RTC Compiler.chain Source.sem Target.sem trel.
+  Corollary extra_target_RTCt : rel_RTC Compiler.chain Source.sem Target.sem trel.
   Proof.
     unfold rel_RTC. simpl. intros par_s ctx_t t Hsem.
     exists (clean_ctx ctx_t), (clean_trace t). split.
-    - now apply trel_clean_trace.
+    - eapply trel_clean_trace; eassumption.
     - now apply sem_clean.
   Qed.
 End RTCtilde.
